\documentclass{article}
\usepackage[utf8]{inputenc}
\usepackage{lipsum}
% Add your standard macros here
\begin{document}
\n\n% --------------------------------------------------------------\n%                         Start here\n% --------------------------------------------------------------\n\n\\title{Math Assignment: Understanding Basic Algebraic Equations}\n\\author{Name of Student\\\\ %replace with your name\nCourse Title, Semester}\n\n\\maketitle\n\n\\noindent For this assignment, I will solve the following basic algebraic equations:\n\n1. \\(2x + 3 = 7\\)\n2. \\(\\frac{4y - 5}{6} = 2\\)\n\nFirst, let's solve the equation for \\(x\\) in part (a):\n\n\\[\n2x + 3 = 7\n\\]\n\nSubtract 3 from both sides:\n\n\\[\n2x = 7 - 3\n\\]\n\\[\n2x = 4\n\\]\n\nDivide both sides by 2:\n\n\\[\nx = \\frac{4}{2}\n\\]\n\\[\nx = 2\n\\]\n\nSo, the solution for part (a) is \\( x = 2 \\).\n\nNext, let's solve the equation for \\(y\\) in part (b):\n\n\\[\n\\frac{4y - 5}{6} = 2\n\\]\n\nMultiply both sides by 6 to eliminate the fraction:\n\n\\[\n4y - 5 = 12\n\\]\n\nAdd 5 to both sides:\n\n\\[\n4y = 12 + 5\n\\]\n\\[\n4y = 17\n\\]\n\nDivide both sides by 4:\n\n\\[\ny = \\frac{17}{4}\n\\]\n\\[\ny = 4.25\n\\]\n\nSo, the solution for part (b) is \\( y = 4.25 \\).\n\nLet's check our solutions by substituting them back into the original equations.\n\nFor part (a):\n\n\\[\n2x + 3 = 7\n\\]\n\\[\n2(2) + 3 = 7\n\\]\n\\[\n4 + 3 = 7\n\\]\n\\[\n7 = 7 \\quad (\\text{True})\n\\]\n\nSo, \\( x = 2 \\) is correct.\n\nFor part (b):\n\n\\[\n\\frac{4y - 5}{6} = 2\n\\]\n\\[\n\\frac{4(4.25) - 5}{6} = 2\n\\]\n\\[\n\\frac{17 - 5}{6} = 2\n\\]\n\\[\n\\frac{12}{6} = 2\n\\]\n\\[\n2 = 2 \\quad (\\text{True})\n\\]\n\nSo, \\( y = 4.25 \\) is correct.\n\nTherefore, the solutions are:\n- For part (a): \\( x = 2 \\)\n- For part (b): \\( y = 4.25 \\)\n\n% --------------------------------------------------------------\n\n\
\end{document}
